Refactor definitions, note proof obligation gap
Block-to-compartment correspondence is tighter than other proof
obligations, which could complicate the task to some degree.

security/Recomposition.v
@@ -125,13 +125,16 @@ Fixpoint merge_stacks (s s'' : stack) : stack :=
    to reflect the mapping, i.e., the same mapping must be applied to block
    identifiers in pointer values. *)
 
-Definition remap {X : Type} (s : side) (t : Maps.PTree.t X) (e : positive * X) : Maps.PTree.t X :=
+(* TODO Add side filtering *)
+Definition remap
+  {X : Type} (s : side) (f : X -> X)
+  (t : Maps.PTree.t X) (e : positive * X) : Maps.PTree.t X :=
   let '(b, x) := e in
   let b' := match s with
             | Left => 2 * b
             | Right => 2 * b + 1
             end%positive in
-  Maps.PTree.set b' x t.
+  Maps.PTree.set b' (f x) t.
 
 (* TODO Actually go from [memval] to [val], remap blocks according to the side
    and leave the rest intact (see [memory_chunk], [AST]) *)
@@ -140,38 +143,28 @@ Definition merge_value (s : side) (v : memval) : memval :=
 
 Definition merge_contents (m m'' : mem) :=
   let (def, c) := Mem.mem_contents m in
-  let (def'', c'') := Mem.mem_contents m'' in
-  (* let set_left t '(b, o2mv) := Maps.PTree.set (2 * b) o2mv t in (* TODO Merge values *) *)
-  (* let set_right t '(b, o2mv) := Maps.PTree.set (2 * b + 1) o2mv t in (* TODO Merge values *) *)
-  (* let celts := Maps.PTree.elements c in *)
-  (* let celts'' := Maps.PTree.elements c'' in *)
-  (* let _ := List.fold_left (fun acc '(b, y) => Maps.PTree.set b y acc) celts (Maps.PTree.empty _) in *)
-  (* not there yet? -- filter things not in left/right! *)
-  let t0 := List.fold_left (remap Left) (Maps.PTree.elements c) (Maps.PTree.empty _) in
-  let t1 := List.fold_left (remap Right) (Maps.PTree.elements c'') t0 in
+  let (_, c'') := Mem.mem_contents m'' in (* default discarder *)
+  (* TODO Filter according to side *)
+  let t0 := List.fold_left (remap Left id) (Maps.PTree.elements c) (Maps.PTree.empty _) in
+  let t1 := List.fold_left (remap Right id) (Maps.PTree.elements c'') t0 in
   (def, t1).
-  (* TODO Not a pure map function *)
-  (* m. *)
-  (* let cnew := Maps.PMap.map (Maps.ZMap.map (merge_value Left)) c in *)
-  (* let cnew'' := Maps.PMap.map (Maps.ZMap.map (merge_value Left)) c'' in *)
-  (* cnew. (* TODO Merge [cnew] and [cnew''] *) *)
 
 Definition merge_access (m m'' : mem) :=
   let '(def, a) := Mem.mem_access m in
-  let '(def'', a'') := Mem.mem_access m'' in (* default discarded *)
-  (* TODO Remap and combine block identifiers according to side *)
-  let t0 := List.fold_left (remap Left) (Maps.PTree.elements a) (Maps.PTree.empty _) in
-  let t1 := List.fold_left (remap Right) (Maps.PTree.elements a'') t0 in
+  let '(_, a'') := Mem.mem_access m'' in (* default discarded *)
+  (* TODO Filter according to side *)
+  let t0 := List.fold_left (remap Left id) (Maps.PTree.elements a) (Maps.PTree.empty _) in
+  let t1 := List.fold_left (remap Right id) (Maps.PTree.elements a'') t0 in
   (def, t1).
 
-
+(* TODO Compartments must be assigned to all "allocated" blocks:
+   [Plt b (merge_nextblocks m m'')] *)
 Definition merge_compartments (m m'' : mem) :=
   let c := Mem.mem_compartments m in
   let c'' := Mem.mem_compartments m'' in
-  (* TODO Remap and combine block identifiers according to side
-     Filter *)
-  let t0 := List.fold_left (remap Left) (Maps.PTree.elements c) (Maps.PTree.empty _) in
-  let t1 := List.fold_left (remap Right) (Maps.PTree.elements c'') t0 in
+  (* TODO Filter according to side *)
+  let t0 := List.fold_left (remap Left id) (Maps.PTree.elements c) (Maps.PTree.empty _) in
+  let t1 := List.fold_left (remap Right id) (Maps.PTree.elements c'') t0 in
   t1.
 
 Definition merge_nextblocks (m m'' : mem) :=
@@ -187,6 +180,10 @@ Program Definition merge_memories (m m'' : mem) : mem :=
    ; Mem.nextblock := merge_nextblocks m m''
   |}.
 Next Obligation.
+Proof.
+  unfold Mem.perm_order'', merge_access.
+  destruct m as [A [def mem_access] C D access_max F G H]; simpl; clear A C D F G H.
+  destruct m'' as [A [def'' mem_access''] C D access_max'' F G H]; simpl; clear A C D F G H.
 Admitted.
 Next Obligation.
 Admitted.
